src/ml/libvellvm/interpreter.mli
@@ -3,12 +3,12 @@ open ITreeDefinition
 
 val pp_addr : Format.formatter -> Memory.A.addr -> unit
 
-val pp_dvalue : Format.formatter -> DV.dvalue -> unit
+val pp_uvalue : Format.formatter -> DV.uvalue -> unit
 
-val interpret: ((LLVMAst.typ, (LLVMAst.typ LLVMAst.block) list) LLVMAst.toplevel_entity) list -> (DV.dvalue, string) result
+val interpret: ((LLVMAst.typ, (LLVMAst.typ LLVMAst.block) list) LLVMAst.toplevel_entity) list -> (DV.uvalue, string) result
 
 (* SAZ: do we need to expose the step function in this way?  Its type is very complicated *)
 (* val step : ((Obj.t Std.failureE, Obj.t debugE, 'b) Sum.sum1, DV.dvalue) coq_LLVM -> (TopLevel.IO.DV.dvalue, string) result *)
-val step : ('a TopLevel.IO.coq_L5, TopLevel.TopLevelEnv.memory * ((TopLevel.TopLevelEnv.local_env * TopLevel.TopLevelEnv.stack) * (TopLevel.TopLevelEnv.global_env * TopLevel.IO.DV.dvalue))) itree -> (TopLevel.IO.DV.dvalue, string) result
+val step : ('a TopLevel.IO.coq_L5, TopLevel.TopLevelEnv.memory * ((TopLevel.TopLevelEnv.local_env * TopLevel.TopLevelEnv.stack) * (TopLevel.TopLevelEnv.global_env * TopLevel.IO.DV.uvalue))) itree -> (TopLevel.IO.DV.uvalue, string) result
 
 val debug_flag: bool ref
