src/coq/TopLevelRefinements.v
@@ -7,6 +7,7 @@ From ITree Require Import
      Eq.Eq.
 
 From Vellvm Require Import
+     DynamicTypes
      CFG
      Memory
      Refinement
@@ -15,12 +16,14 @@ From Vellvm Require Import
      LLVMAst
      Handlers.Global
      Handlers.Local
-     Handlers.Stack.
+     Handlers.Stack
+     Handlers.UndefinedBehaviour.
 
 From ExtLib Require Import
      Structures.Functor.
 
 From Coq Require Import
+     Strings.String
      Logic
      Morphisms
      Relations
@@ -32,6 +35,17 @@ Import ITree.Basics.Basics.Monads.
 Module R := Refinement.Make(Memory.A)(IO)(TopLevelEnv).
 Import R.
 Import TopLevelEnv.
+
+(**
+   YZ: Trying to figure how to tidy up everything. This file is currently a holdall.
+   In here, we have:
+   * partial interpreters to each levels;
+   * hierarchies of refinements of mcfgs and proofs of inclusions;
+   * lemmas for each partial interpreter of commutation with bind and ret;
+   * some misc proper instances;
+   * admitted statement of inclusion of the intepreter into the model;
+ **)
+
 
 (** The module _Refinement.Make_ defines a series of refinements between
     [itree]s at the various signatures of events a Vellvm goes through during
@@ -105,34 +119,34 @@ Qed.
     refinement at level [i+1] after running the [i+1] level of interpretation
  *)
 
-Lemma refine_01: forall t1 t2,
-    refine_L0 t1 t2 -> refine_L1 (build_L1 t1) (build_L1 t2).
+Lemma refine_01: forall t1 t2 g,
+    refine_L0 t1 t2 -> refine_L1 (run_state (interp_global t1) g) (run_state (interp_global t2) g).
 Proof.
-  intros t1 t2 H.
+  intros t1 t2 g H.
   apply eutt_tt_to_eq_prod, eutt_interp_state_gen; auto.
 Qed.
 
-Lemma refine_12 : forall t1 t2,
-    refine_L1 t1 t2 -> refine_L2 (build_L2 t1) (build_L2 t2).
+Lemma refine_12 : forall t1 t2 l,
+    refine_L1 t1 t2 -> refine_L2 (run_state (interp_local_stack (handle_local (v:=res_L0)) t1) l) (run_state (interp_local_stack (handle_local (v:=res_L0)) t2) l).
 Proof.
-  intros t1 t2 H.
+  intros t1 t2 l H.
   apply eutt_tt_to_eq_prod, eutt_interp_state_gen; auto.
 Qed.
 
-Lemma refine_23 : forall t1 t2,
-    refine_L2 t1 t2 -> refine_L3 (build_L3 t1) (build_L3 t2).
+Lemma refine_23 : forall t1 t2 m,
+    refine_L2 t1 t2 -> refine_L3 (run_state (M.interp_memory t1) m) (run_state (M.interp_memory t2) m).
 Proof.
-  intros t1 t2 H.
+  intros t1 t2 m H.
   apply eutt_tt_to_eq_prod, eutt_interp_state_gen; auto.
 Qed.
 
 (* Things are different for L4 and L5: we get into the [Prop] monad. *)
 Lemma refine_34 : forall t1 t2,
-    refine_L3 t1 t2 -> refine_L4 (model_L4 t1) (model_L4 t2).
+    refine_L3 t1 t2 -> refine_L4 (P.model_undef t1) (P.model_undef t2).
 Proof.
   intros t1 t2 H t Ht.
   exists t; split.
-  - unfold model_L4, P.model_undef in *.
+  - unfold P.model_undef in *.
     unfold IO.L3 in *.
     match goal with |- PropT.interp_prop ?x _ _ _ => remember x as h end.
     eapply interp_prop_Proper; eauto.
@@ -140,7 +154,7 @@ Proof.
 Qed.
 
 Lemma refine_45 : forall Pt1 Pt2,
-    refine_L4 Pt1 Pt2 -> refine_L5 (model_L5 Pt1) (model_L5 Pt2).
+    refine_L4 Pt1 Pt2 -> refine_L5 (model_UB Pt1) (model_UB Pt2).
 Proof.
   intros Pt1 Pt2 HR t2 HM.
   exists t2; split; [| reflexivity].
@@ -152,165 +166,322 @@ Proof.
 Qed.
 
 (**
-   We now define partial interpretations in order to define refinements of [mcfg]s
+   We now define partial interpretations of the trees produced by the
+   denotation of vellvm programs.
+   The intent is to allow us to only interpret as many layers as needed
+   to perform the required semantic reasoning, and lift for free the
+   equivalence down the pipe.
+   This gives us a _vertical_ notion of compositionality.
  *)
 
-Definition interp_to_L1 {R} (t: itree IO.L0 R) g :=
-  let L0_trace       := INT.interpret_intrinsics nil t in
+Definition interp_to_L1 {R} user_intrinsics (t: itree IO.L0 R) g :=
+  let L0_trace       := INT.interpret_intrinsics user_intrinsics t in
   let L1_trace       := run_state (interp_global L0_trace) g in
   L1_trace.
 
-Definition build_to_L1 (prog: mcfg typ) :=
-  let mcfg := normalize_types prog in
-  let L0_trace        := denote_vellvm mcfg in
-  interp_to_L1 L0_trace [].
-
-Definition interp_to_L2 {R} (t: itree IO.L0 R) g l :=
-  let L0_trace       := INT.interpret_intrinsics [] t in
+Definition interp_to_L2 {R} user_intrinsics (t: itree IO.L0 R) g l :=
+  let L0_trace       := INT.interpret_intrinsics user_intrinsics t in
   let L1_trace       := run_state (interp_global L0_trace) g in
   let L2_trace       := run_state (interp_local_stack (handle_local (v:=res_L0)) L1_trace) l in
   L2_trace.
 
-Definition build_to_L2 (prog: mcfg typ) :=
-  let mcfg := normalize_types prog in
-  let L0_trace        := denote_vellvm mcfg in
-  interp_to_L2 L0_trace [] ([],[]).
-
-Definition interp_to_L3 {R} (t: itree IO.L0 R) g l m :=
-  let L0_trace       := INT.interpret_intrinsics [] t in
+Definition interp_to_L3 {R} user_intrinsics (t: itree IO.L0 R) g l m :=
+  let L0_trace       := INT.interpret_intrinsics user_intrinsics t in
   let L1_trace       := run_state (interp_global L0_trace) g in
   let L2_trace       := run_state (interp_local_stack (handle_local (v:=res_L0)) L1_trace) l in
   let L3_trace       := run_state (M.interp_memory L2_trace) m in
   L3_trace.
 
-Definition build_to_L3 (prog: mcfg typ) :=
-  let mcfg := normalize_types prog in
-  let L0_trace        := denote_vellvm mcfg in
-  interp_to_L3 L0_trace [] ([],[]) (M.empty, [[]]).
-
-Definition build_to_L4 (user_intrinsics: IS.intrinsic_definitions) (prog: mcfg typ) :=
-  let mcfg := normalize_types prog in
-
-  let L0_trace        := denote_vellvm mcfg in
-  let L0_trace'       := INT.interpret_intrinsics user_intrinsics L0_trace in
-  let L1_trace        := build_L1 L0_trace' in
-  let L2_trace        := build_L2 L1_trace in
-  let L3_trace        := build_L3 L2_trace in
-  let L4_trace        := model_L4 L3_trace in
+Definition interp_to_L4 {R} user_intrinsics (t: itree IO.L0 R) g l m :=
+  let L0_trace       := INT.interpret_intrinsics user_intrinsics t in
+  let L1_trace       := run_state (interp_global L0_trace) g in
+  let L2_trace       := run_state (interp_local_stack (handle_local (v:=res_L0)) L1_trace) l in
+  let L3_trace       := run_state (M.interp_memory L2_trace) m in
+  let L4_trace       := P.model_undef L3_trace in
   L4_trace.
 
-Definition refine_mcfg_L1 (p1 p2: mcfg typ): Prop :=
-  R.refine_L1 (build_to_L1 p1) (build_to_L1 p2).
+Ltac fold_L1 :=
+    match goal with
+      |- context[run_state (interp_global (INT.interpret_intrinsics ?ui ?p)) ?g] =>
+      replace (run_state (interp_global (INT.interpret_intrinsics ui p)) g) with
+        (interp_to_L1 ui p g) by reflexivity
+    end.
 
-Definition refine_mcfg_L2 (p1 p2: mcfg typ): Prop :=
-  R.refine_L2 (build_to_L2 p1) (build_to_L2 p2).
+Ltac fold_L2 :=
+    match goal with
+      |- context[
+            run_state
+              (interp_local_stack ?h
+                (run_state (interp_global (INT.interpret_intrinsics ?ui ?p)) ?g)) ?l] =>
+      replace (run_state (interp_local_stack h (run_state (interp_global (INT.interpret_intrinsics ui p)) g)) l) with
+        (interp_to_L2 ui p g l) by reflexivity
+    end.
 
-Definition refine_mcfg_L3 (p1 p2: mcfg typ): Prop :=
-  R.refine_L3 (build_to_L3 p1) (build_to_L3 p2).
+Ltac fold_L3 :=
+    match goal with
+      |- context[
+            run_state (M.interp_memory
+            (run_state
+              (interp_local_stack ?h
+                (run_state (interp_global (INT.interpret_intrinsics ?ui ?p)) ?g)) ?l)) ?m] =>
+      replace (run_state (M.interp_memory (run_state (interp_local_stack h (run_state (interp_global (INT.interpret_intrinsics ui p)) g)) l)) m) with
+        (interp_to_L3 ui p g l m) by reflexivity
+    end.
 
-Definition refine_mcfg_L4 (p1 p2: mcfg typ): Prop :=
-  R.refine_L4 (build_to_L4 nil p1) (build_to_L4 nil p2).
+Ltac fold_L4 :=
+    match goal with
+      |- context[
+            P.model_undef (run_state (M.interp_memory
+            (run_state
+              (interp_local_stack ?h
+                (run_state (interp_global (INT.interpret_intrinsics ?ui ?p)) ?g)) ?l)) ?m)] =>
+      replace (P.model_undef (run_state (M.interp_memory (run_state (interp_local_stack h (run_state (interp_global (INT.interpret_intrinsics ui p)) g)) l)) m)) with
+        (interp_to_L4 ui p g l m) by reflexivity
+    end.
 
-Definition refine_mcfg (p1 p2: mcfg typ): Prop :=
-  R.refine_L5 (model_mcfg p1) (model_mcfg p2).
+Ltac fold_L5 :=
+    match goal with
+      |- context[
+            model_UB (P.model_undef (run_state (M.interp_memory
+            (run_state
+              (interp_local_stack ?h
+                (run_state (interp_global (INT.interpret_intrinsics ?ui ?p)) ?g)) ?l)) ?m))] =>
+      replace (model_UB (P.model_undef (run_state (M.interp_memory (run_state (interp_local_stack h (run_state (interp_global (INT.interpret_intrinsics ui p)) g)) l)) m))) with
+        (interp_vellvm_model_user ui p g l m) by reflexivity
+    end.
 
-Lemma refine_mcfg_L1_correct: forall p1 p2,
-    refine_mcfg_L1 p1 p2 -> refine_mcfg p1 p2.
+(**
+   In particular, we can therefore define top-level models
+   short-circuiting the interpretation early.
+ *)
+Definition model_to_L1 user_intrinsics (prog: mcfg dtyp) :=
+  let L0_trace := denote_vellvm prog in
+  interp_to_L1 user_intrinsics L0_trace [].
+
+Definition model_to_L2 user_intrinsics (prog: mcfg dtyp) :=
+  let L0_trace := denote_vellvm prog in
+  interp_to_L2 user_intrinsics L0_trace [] ([],[]).
+
+Definition model_to_L3 user_intrinsics (prog: mcfg dtyp) :=
+  let L0_trace := denote_vellvm prog in
+  interp_to_L3 user_intrinsics L0_trace [] ([],[]) (M.empty, [[]]).
+
+Definition model_to_L4 user_intrinsics (prog: mcfg dtyp) :=
+  let L0_trace := denote_vellvm prog in
+  interp_to_L4 user_intrinsics L0_trace [] ([],[]) (M.empty, [[]]).
+
+Definition model_to_L5 user_intrinsics (prog: mcfg dtyp) :=
+  let L0_trace := denote_vellvm prog in
+  interp_vellvm_model_user user_intrinsics L0_trace [] ([],[]) (M.empty, [[]]).
+
+(**
+   Which leads to five notion of equivalence of [mcfg]s.
+   Note that all reasoning is conducted after conversion to [mcfg] and
+   normalization of types.
+ *)
+Definition refine_mcfg_L1 user_intrinsics (p1 p2: mcfg dtyp): Prop :=
+  R.refine_L1 (model_to_L1 user_intrinsics p1) (model_to_L1 user_intrinsics p2).
+
+Definition refine_mcfg_L2 user_intrinsics (p1 p2: mcfg dtyp): Prop :=
+  R.refine_L2 (model_to_L2 user_intrinsics p1) (model_to_L2 user_intrinsics p2).
+
+Definition refine_mcfg_L3 user_intrinsics (p1 p2: mcfg dtyp): Prop :=
+  R.refine_L3 (model_to_L3 user_intrinsics p1) (model_to_L3 user_intrinsics p2).
+
+Definition refine_mcfg_L4 user_intrinsics (p1 p2: mcfg dtyp): Prop :=
+  R.refine_L4 (model_to_L4 user_intrinsics p1) (model_to_L4 user_intrinsics p2).
+
+Definition refine_mcfg user_intrinsics  (p1 p2: mcfg dtyp): Prop :=
+  R.refine_L5 (model_to_L5 user_intrinsics p1) (model_to_L5 user_intrinsics p2).
+
+(**
+   The chain of refinements is monotone, legitimating the ability to
+   conduct reasoning before interpretation when suitable.
+ *)
+Lemma refine_mcfg_L1_correct: forall user_intrinsics p1 p2,
+    refine_mcfg_L1 user_intrinsics p1 p2 -> refine_mcfg user_intrinsics p1 p2.
 Proof.
-  intros p1 p2 HR.
+  intros ? p1 p2 HR.
   apply refine_45, refine_34, refine_23, refine_12, HR.
 Qed.
 
-Lemma refine_mcfg_L2_correct: forall p1 p2,
-    refine_mcfg_L2 p1 p2 -> refine_mcfg p1 p2.
+Lemma refine_mcfg_L2_correct: forall user_intrinsics p1 p2,
+    refine_mcfg_L2 user_intrinsics p1 p2 -> refine_mcfg user_intrinsics p1 p2.
 Proof.
-  intros p1 p2 HR.
+  intros ? p1 p2 HR.
   apply refine_45, refine_34, refine_23, HR.
 Qed.
 
-Lemma refine_mcfg_L3_correct: forall p1 p2,
-    refine_mcfg_L3 p1 p2 -> refine_mcfg p1 p2.
+Lemma refine_mcfg_L3_correct: forall user_intrinsics p1 p2,
+    refine_mcfg_L3 user_intrinsics p1 p2 -> refine_mcfg user_intrinsics p1 p2.
 Proof.
-  intros p1 p2 HR.
+  intros ? p1 p2 HR.
   apply refine_45, refine_34, HR.
 Qed.
 
-Lemma refine_mcfg_L4_correct: forall p1 p2,
-    refine_mcfg_L4 p1 p2 -> refine_mcfg p1 p2.
+Lemma refine_mcfg_L4_correct: forall user_intrinsics p1 p2,
+    refine_mcfg_L4 user_intrinsics p1 p2 -> refine_mcfg user_intrinsics p1 p2.
 Proof.
-  intros p1 p2 HR.
+  intros ? p1 p2 HR.
   apply refine_45, HR.
 Qed.
 
-(* TODO SCRAPYARD, TO RECYCLE OR BURN
-Instance refine_uvalue_refl :
-  Reflexive refine_uvalue.
-Proof.
-  unfold Reflexive. intros x.
-  induction x; constructor; auto.
-Qed.
+(* MOVE *)
+Ltac flatten_goal :=
+  match goal with
+  | |- context[match ?x with | _ => _ end] => let Heq := fresh "Heq" in destruct x eqn:Heq
+  end.
 
-Instance TT_refl :
-  forall A, Reflexive (@TT A).
-Proof.
-  firstorder.
-Qed.
+Ltac flatten_hyp h :=
+  match type of h with
+  | context[match ?x with | _ => _ end] => let Heq := fresh "Heq" in destruct x eqn:Heq
+  end.
 
-Lemma model_refines :
-  forall t1 t, (model_L4 t1) t -> refine_L4 (fun t' => t = t') (model_L4 t1).
-Proof.
-  intros t1 t H.
-  unfold refine_L4. intros t' Heq.
-  exists t. split; auto.
-  subst.
+Ltac flatten_all :=
+  match goal with
+  | h: context[match ?x with | _ => _ end] |- _ => let Heq := fresh "Heq" in destruct x eqn:Heq
+  | |- context[match ?x with | _ => _ end] => let Heq := fresh "Heq" in destruct x eqn:Heq
+  end.
 
-  apply Reflexive_eqit.
-  repeat apply prod_rel_refl; auto using TT_refl, refine_uvalue_refl.
-Qed.
-*)
-
-(* Unfinished proof *)
-(*
-Lemma refine_34_concrete : forall t1 t2,
-    refine_L3 t1 t2 -> refine_L4_concrete (build_L4 t1) (build_L4 t2).
-Proof.
-  intros t1 t2 H.
-  unfold refine_L4_concrete.
-  unfold refine_L3 in H.
-
-  eapply eqit_mon.
-  apply id. apply id.
-
-  intros x0 x1 PR.
-  unfold refine_res4.
-  eapply subrelation_prod_left. apply subrelation_R_TT with (R:=eq). apply PR.
-
-Qed.
+(**
+   We should be able to prove that the interpreter belongs to the model.
  *)
-
-(*
-Lemma refine_45 : forall t1 t2,
-    refine_L4 t1 t2 -> refine_L5 (model_L5 t1) (model_L5 t2).
+Theorem interpreter_sound: forall p, model p (interpreter p).
 Proof.
-  intros t1 t2 H.
-  unfold refine_L5.
-  intros t Hip.
+  intros p.
+  unfold model, model_user.
+  flatten_goal.
+  2:{
+    unfold interpreter, interpreter_user.
+    rewrite Heq; reflexivity.
+  }
+  unfold interpreter, interpreter_user; rewrite Heq.
+  unfold interp_vellvm_model_user, interp_vellvm_exec_user.
+  match goal with |- model_UB _ (interp_UB ?t) => exists t end.
+  split.
+  {
+    fold_L4.
+    admit.
+  }
+  admit.
+Admitted.
 
-  exists t. split.
-  - unfold model_L5 in *.
-    unfold UndefinedBehaviour.model_UB in *.
-    destruct Hip as [t' [t1p Hip]].
+(**
+   Each interpreter commutes with [bind] and [ret].
+ **)
 
-    exists t'. split.
-    + unfold refine_L4 in H.
-      pose proof (H t' t1p) as H1.
-      destruct H1 as [t'' [Ht2t'' Ht't'']].
-
-      Print Basics.impl.
-      rewrite Ht't''.
-    + apply Hip.
-  - reflexivity.
-
-  repeat apply prod_rel_refl; auto using TT_refl, refine_uvalue_refl.
+(* This should move to the library. It's just a specialization of [eqit_bind'], but I like the much more
+ informative name. *)
+From ExtLib Require Import
+     Structures.Monads.
+Import MonadNotation.
+Lemma eq_itree_clo_bind {E : Type -> Type} {R1 R2 : Type} (RR : R1 -> R2 -> Prop) {U1 U2 UU} t1 t2 k1 k2
+      (EQT: @eq_itree E U1 U2 UU t1 t2)
+      (EQK: forall u1 u2, UU u1 u2 -> eq_itree RR (k1 u1) (k2 u2)):
+  eq_itree RR (x <- t1;; k1 x) (x <- t2;; k2 x).
+Proof.
+  eapply eqit_bind'; eauto.
 Qed.
- *)
+
+Lemma interp_intrinsics_bind :
+  forall (R S : Type) l (t : itree _ R) (k : R -> itree _ S),
+    INT.interpret_intrinsics l (ITree.bind t k) ≅ ITree.bind (INT.interpret_intrinsics l t) (fun r : R => INT.interpret_intrinsics l (k r)).
+Proof.
+  intros; apply interp_bind.
+Qed.
+
+Lemma interp_intrinsics_ret :
+  forall (R : Type) l (x: R),
+    INT.interpret_intrinsics l (Ret x) ≅ Ret x.
+Proof.
+  intros; apply interp_ret.
+Qed.
+
+Lemma interp_global_bind :
+  forall (R S : Type) (t : itree IO.L0 R) (k : R -> itree IO.L0 S) s,
+    run_state (interp_global (ITree.bind t k)) s ≅
+              ITree.bind (run_state (interp_global t) s) (fun '(s',r) => run_state (interp_global (k r)) s').
+Proof.
+  intros.
+  unfold interp_global.
+  setoid_rewrite interp_state_bind.
+  apply eq_itree_clo_bind with (UU := Logic.eq).
+  reflexivity.
+  intros [] [] EQ; inv EQ; reflexivity.
+Qed.
+
+Lemma interp_global_ret :
+  forall (R : Type) g (x: R),
+    run_state (interp_global (Ret x: itree IO.L0 R)) g ≅ Ret (g,x).
+Proof.
+  intros; apply interp_state_ret.
+Qed.
+
+Lemma interp_local_stack_bind :
+  forall (R S: Type) (t : itree IO.L1 _) (k : R -> itree IO.L1 S) s,
+    run_state (interp_local_stack (handle_local (v:=res_L0)) (ITree.bind t k)) s ≅
+              ITree.bind (run_state (interp_local_stack (handle_local (v:=res_L0)) t) s)
+              (fun '(s',r) => run_state (interp_local_stack (handle_local (v:=res_L0)) (k r)) s').
+Proof.
+  intros.
+  unfold interp_local_stack.
+  setoid_rewrite interp_state_bind.
+  apply eq_itree_clo_bind with (UU := Logic.eq).
+  reflexivity.
+  intros [] [] EQ; inv EQ; reflexivity.
+Qed.
+
+Lemma interp_local_stack_ret :
+  forall (R : Type) l (x: R),
+    run_state (interp_local_stack (handle_local (v:=uvalue)) (Ret x: itree IO.L1 R)) l ≅ Ret (l,x).
+Proof.
+  intros; apply interp_state_ret.
+Qed.
+
+(** We hence can also commute them at the various levels of interpretation *)
+
+(** BEGIN MOVE *)
+From ITree Require Import
+     Events.StateKleisli
+     Events.StateFacts.
+
+Instance run_state_proper_eqit {E A env} : Proper (MonadTheory.eqm ==> Logic.eq ==> eutt Logic.eq) (@run_state E A env).
+Proof.
+  repeat intro; subst; apply H.
+Qed.
+
+Require Import Paco.paco.
+Instance interp_state_proper {T E F S} (h: forall T : Type, E T -> Monads.stateT S (itree F) T) : Proper (eutt Logic.eq ==> MonadTheory.eqm) (State.interp_state h (T := T)).
+Proof.
+  einit. ecofix CIH. intros.
+
+  rewrite !unfold_interp_state. punfold H0. red in H0.
+  induction H0; intros; subst; simpl; pclearbot.
+  - eret.
+  - etau.
+  - ebind. econstructor; [reflexivity|].
+    intros; subst.
+    etau. ebase.
+  - rewrite tau_eutt, unfold_interp_state; eauto.
+  - rewrite tau_eutt, unfold_interp_state; eauto.
+Qed.
+
+(** END MOVE *)
+
+Lemma interp_to_L2_bind:
+  forall ui {R S} (t: itree IO.L0 R) (k: R -> itree IO.L0 S) s1 s2,
+    interp_to_L2 ui (ITree.bind t k) s1 s2 ≈
+                 (ITree.bind (interp_to_L2 ui t s1 s2) (fun '(s1',(s2',x)) => interp_to_L2 ui (k x) s2' s1')).
+Proof.
+  intros.
+  unfold interp_to_L2.
+  rewrite interp_intrinsics_bind, interp_global_bind, interp_local_stack_bind.
+  apply eutt_clo_bind with (UU := Logic.eq); [reflexivity | intros ? (? & ? & ?) ->; reflexivity].
+Qed.
+
+Lemma interp_to_L2_ret: forall ui (R : Type) s1 s2 (x : R), interp_to_L2 ui (Ret x) s1 s2 ≈ Ret (s2, (s1, x)).
+Proof.
+  intros; unfold interp_to_L2.
+  rewrite interp_intrinsics_ret, interp_global_ret, interp_local_stack_ret; reflexivity.
+Qed.
+
