src/coq/Transformations/SubstCFG.v
@@ -1,0 +1,196 @@
+From Coq Require Import
+     ZArith Ascii Strings.String Setoid Morphisms List.
+
+From ExtLib Require Import
+     Programming.Eqv
+     Structures.Monads.
+
+From ITree Require Import
+     ITree
+     Eq.Eq
+     Interp.Interp
+     Interp.InterpFacts
+     Interp.TranslateFacts
+     Events.StateKleisli
+     Events.StateFacts.
+
+From Vellvm Require Import
+     PropT
+     Error
+     Util
+     LLVMAst
+     AstLib
+     CFG
+     TransformTypes
+     DynamicTypes
+     DynamicValues
+     Denotation
+     Handlers.Global
+     Handlers.Local
+     Handlers.Stack
+     Handlers.Memory
+     Handlers.UndefinedBehaviour
+     LLVMEvents
+     Transformations.Transformation
+     Traversal
+     TopLevelRefinements.
+
+Import ListNotations.
+Import TopLevel.
+Import TopLevelEnv.
+Import R.
+Import EqvNotation.
+
+(* WIP, broken, not compiled by the makefile **)
+
+(* -------------------------------------------------- *)
+(* CFG substitution into MCFG.                       *)
+(* -------------------------------------------------- *)
+
+Section Substitute_cfg.
+
+  Context {T : Set}.
+  Variable fid: function_id.
+  Variable new_f : cfg T.
+
+  (* This assumes the new function shares the exact same prototype. *)
+  Instance subst_cfg_endo_cfg: endo (definition T (cfg T)) :=
+    fun f => if (dc_name (df_prototype f)) ~=? fid
+          then {| df_prototype := df_prototype f; df_args := df_args f ; df_instrs := new_f |}
+          else f.
+
+  Definition subst_cfg: endo (mcfg T) := f_endo.
+
+End Substitute_cfg.
+
+Definition interpret_model (t: itree IO.L0 res_L0): PropT (itree IO.L5) res_L3 :=
+  let L0_trace        := INT.interpret_intrinsics [] t in
+  let L1_trace        := run_state (interp_global L0_trace) [] in
+  let L2_trace        := run_state (interp_local_stack (@handle_local _ _ _ _ _ _ _) L1_trace) ([],[]) in
+  let L3_trace        := run_state (M.interp_memory L2_trace) (M.empty, [[]]) in
+  let L4_trace        := model_L4 L3_trace in
+  let L5_trace        := model_L5 L4_trace in
+  L5_trace.
+
+
+Definition model_mcfg_user' (user_intrinsics: IS.intrinsic_definitions) (prog: CFG.mcfg dtyp) : PropT (itree IO.L5) res_L3 :=
+  let L0_trace        := denote_vellvm prog in
+  let L0_trace'       := INT.interpret_intrinsics user_intrinsics L0_trace in
+  let L1_trace        := run_state (interp_global L0_trace') [] in
+  let L2_trace        := run_state (interp_local_stack (@handle_local _ _ _ _ _ _ _) L1_trace) ([],[]) in
+  let L3_trace        := run_state (M.interp_memory L2_trace) (M.empty, [[]]) in
+  let L4_trace        := model_L4 L3_trace in
+  let L5_trace        := model_L5 L4_trace in
+  L5_trace.
+
+Definition transformation_correct (T: endo (mcfg dtyp)) p: Prop :=
+  refine_L5 (model_mcfg_user' [] p) (model_mcfg_user' [] (T p)).
+
+(* Definition model_to_L5 {R E} (t: itree IO.L0 R) g l m := *)
+(*   let L0_trace       := INT.interpret_intrinsics [] t in *)
+(*   let L1_trace       := run_state (interp_global L0_trace) g in *)
+(*   let L2_trace       := run_state (interp_local_stack (handle_local (v:=res_L0)) L1_trace) l in *)
+(*   let L3_trace       := run_state (M.interp_memory L2_trace) m in *)
+(*   let L4_trace       := P.model_undef L3_trace in *)
+(*   let L5_trace       := model_UB L4_trace *)
+(*   in L5_trace. *)
+
+
+Section Substitute_cfg_correct.
+
+  Lemma subst_cfg_correct:
+    forall (p: mcfg dtyp) id f d,
+      In d (m_definitions p) ->
+      dc_name (df_prototype d) = id ->
+      model_cfg (D.denote_cfg (df_instrs d)) (D.denote_cfg f) ->
+      transformation_correct (subst_cfg id f) p.
+  Proof.
+    intros.
+    remember (D.denote_cfg f).
+
+    intros p.
+    unfold refine_mcfg_L2.
+    unfold build_to_L2.
+
+    (* Proof obligation number 1: commutation with normalize_types. *)
+    rewrite normalize_types_swap.
+    pattern (normalize_types p); generalize (normalize_types p); clear p; intros p.
+
+    unfold denote_vellvm.
+    simpl; rewrite 2 interp_to_L2_bind.
+    split_bind.
+
+    {
+      (* Reasoning about initialization *)
+      admit.
+    }
+
+    rewrite 2 interp_to_L2_bind.
+    apply eutt_clo_bind with foo_rel.
+
+    {
+      (* Denotation of each cfg *)
+      apply interp_to_L2_map_monad.
+      admit.
+    }
+
+    intros (? & ? & ?) (? & ? & ?) EQ.
+    inv EQ; repeat match goal with | h: prod_rel _ _ _ _ |- _ => inv h end.
+    rewrite 2 interp_to_L2_bind.
+    split_bind.
+
+    { (* Getting the address of "main" *)
+      admit.
+    }
+
+    (* Tying the recursive knot *)
+
+    admit.
+  (*   rewrite 2 interp_to_L2_bind. *)
+
+
+
+
+(* -------------------------------------------------- *)
+(* Block substitution into CFG.                       *)
+(* -------------------------------------------------- *)
+
+Section Substitute_block.
+
+  Variable T : Set.
+  Variable b : block T.
+
+
+
+Fixpoint replace_pred {A} (p : A -> bool) (a : A) (xs : list A) : list A :=
+  match xs with
+  | nil => nil
+  | (x::xs') =>
+    if p x
+    then a :: xs'
+    else x :: replace_pred p a xs'
+  end.
+
+From ExtLib Require Import
+     Core.RelDec
+     Programming.Eqv.
+
+
+(* Replace a block with a given block r if the ids match *)
+Definition replace_block {T} (r : block T) (b : block T) : block T :=
+  if blk_id b ~=? blk_id r then r else b.
+
+Section block_replace.
+  Variable T : Set.
+  Variable b : block T.
+
+  Definition blah := b.
+
+  Instance block_replace_endo : endo (block T)
+    := replace_block b.
+
+  Definition cfg_replace_block : endo (cfg T)
+    := f_endo.
+End block_replace.
+
+
